finally finished a working parser for s-expressions

ParsingNative.cs
@@ -1,10 +1,143 @@
+using System;
 using System.IO;
+using Dafny;
 
 namespace @_0_Parsing_Compile {
-  public partial class @FileSystem {
-    public static void ReadFile(char[] fname, out char[] result) {
-      string sname = new string(fname);
-      result = File.ReadAllText(sname).ToCharArray();
+  public partial class Option<A> {
+    private readonly A val;
+    private readonly bool isNone;
+    public Option(A a) {
+      this.val = a;
+      this.isNone = false;
+    }
+    public Option() {
+      this.isNone = true;
+    }
+    public bool IsNone() { return isNone; }
+    public A Val() { return val; }
+    public override string ToString() {
+      if (isNone) {
+        return "None";
+      } else {
+        return "Some(" + val.ToString() + ")";
+      }
+    }
+  }
+
+  public partial class Parser<A> {
+    internal readonly Func<string, Tuple<A, string>> p;
+
+    internal Parser(Func<string, Tuple<A, string>> p) {
+      this.p = p;
+    }
+
+    public Parser<B> Map<B>(Func<A, B> f) {
+      return new Parser<B>(s => {
+        Tuple<A, string> t = p(s);
+        return t == null ? null : Tuple.Create(f(t.Item1), t.Item2);
+      });
+    }
+
+    public Parser<A> Or(Parser<A> p2) {
+      return new Parser<A>(s => {
+        Tuple<A, string> r = p(s);
+        return r == null ? p2.p(s): r;
+      });
+    }
+
+    public Parser<B> Bind<B>(Func<A, Parser<B>> f) {
+      return new Parser<B>(s => {
+        Tuple<A, string> r = p(s);
+        if (r == null) return null;
+        Parser<B> pb = f(r.Item1);
+        return pb.p(r.Item2);
+      });
+    }
+
+    public Parser<C> Seq<B,C>(Parser<B> pb, Func<A, B, C> f) {
+      return Bind(a => {
+        return pb.Bind(b => @_0_Parsing_Compile.Parse.Const(f(a,b)));
+      });
+    }
+
+    public Parser<A> Skip<B>(Parser<B> pb) {
+      return Seq(pb, (a,b) => a);
+    }
+
+    public Parser<B> Then<B>(Parser<B> pb) {
+      return Seq(pb, (a,b) => b);
+    }
+
+    public Parser<A> SkipWS() {
+      Parser<Sequence<char>> ws = @_0_Parsing_Compile.Parse.Char(' ')
+        .Or(@_0_Parsing_Compile.Parse.Char('\t'))
+        .Or(@_0_Parsing_Compile.Parse.Char('\n')).ZeroOrMore();
+      return ws.Then(Skip(ws));
+    }
+
+    public Parser<Sequence<A>> ZeroOrMore() {
+      return OneOrMore().Or(@_0_Parsing_Compile.Parse.Const(Sequence<A>.Empty));
+    }
+
+    public Parser<Sequence<A>> OneOrMore() {
+      return Bind<Sequence<A>>(a =>
+        ZeroOrMore().Bind<Sequence<A>>(aa =>
+          @_0_Parsing_Compile.Parse.Const(
+            Sequence<A>.FromElements(a).Concat(aa))));
+    }
+
+    private Option<A> Parse(string str) {
+      Tuple<A, string> t = p(str.ToString());
+      return t == null || !string.IsNullOrEmpty(t.Item2)
+        ? new Option<A>()
+          : new Option<A>(t.Item1);
+    }
+
+    public Option<A> Parse(Sequence<char> str) {
+      return Parse(str.ToString());
+    }
+
+    public Option<A> ParseFile(Sequence<char> filename) {
+      string sname = filename.ToString();
+      return Parse(File.ReadAllText(sname));
+    }
+  }
+
+  public partial class Parse {
+    public static Parser<A> Const<A>(A a) {
+      return new Parser<A>(s => Tuple.Create(a, s));
+    }
+
+    public static Parser<char> SatChar(Func<char, bool> pred) {
+      return new Parser<char>(s => {
+        if (s.Length == 0) {
+          return null;
+        } else if (pred(s[0])) {
+          return Tuple.Create(s[0], s.Substring(1));
+        } else {
+          return null;
+        }
+      });
+    }
+
+    public static Parser<char> Char(char c2) {
+      return SatChar(c => c == c2);
+    }
+
+    public static Parser<char> Digit() {
+      return SatChar(c => '0' <= c && c <= '9');
+    }
+
+    public static Parser<char> Letter() {
+      return SatChar(c => 'A' <= c && c <= 'Z' || 'a' <= c && c <= 'z' || c == '_');
+    }
+
+    /*public static Parser<string> Keyword(string kw) {
+      
+    }*/
+
+    public static Parser<A> Fix<A>(Func<Parser<A>, Parser<A>> f) {
+      return new Parser<A>(s => f(Fix(f)).p(s));
     }
   }
 }
