README.md
@@ -2,11 +2,6 @@
 
 **Parser combinator library for Dafny**
 
-The API is currently based on algebraic datatypes and functions. 
-It would be possible to offer a class/method-based API. However, Dafny
-currently requires a statement based appraoch for imperative code and
-does not allow allocation of (immutable) objects with expressions.
-
 ## Example
 
 ```dafny
@@ -15,9 +10,47 @@ include "Parsing.dfy"
 module Example {
   import opened Parsing
 
+  datatype SExpr = Atom(string) | List(seq<SExpr>)
+
   method Main() {
-    print(Parse(DigitP(), "5")); // Some('5')
-    print(Parse(DigitP(), "X")); // None
+    // single characters
+    var digit: Parser<char> := Parse.Digit();
+    print digit.Parse("5"); // Some(5)
+    print digit.Parse("X"); // None
+    var digitOrLetter: Parser<char> := digit.Or(Parse.Letter());
+    print digitOrLetter.Parse("X"); // Some(X)
+    print digitOrLetter.Parse("+"); // None
+
+    // identifiers
+    var id: Parser<string> := Parse.Letter().Seq(
+                                  digitOrLetter.ZeroOrMore(),
+                                  (c: char, s: string) => [c] + s);
+    print id.Parse("x23"); // Some(x23)
+    print id.Parse("a_s"); // Some(a_s)
+    print id.Parse("12a"); // None
+
+    // s-expressions
+    var sexpr: Parser<SExpr> := Parse.Fix((sexp: Parser<SExpr>) requires sexp != null => (
+      var atom: Parser<SExpr> := digitOrLetter.OneOrMore().Map(s => Atom(s));
+      var lst: Parser<SExpr> :=
+           Parse.Char('(')
+             .Then(sexp.ZeroOrMore().Map(l => List(l)))
+             .Skip(Parse.Char(')'));
+      atom.Or(lst).SkipWS()));
+
+    print sexpr.Parse("x23");     // Some(Atom(x23))
+    print sexpr.Parse("(a b c)"); // Some(List(Atom(a),Atom(b),Atom(c)))
+    print sexpr.Parse("((a) b)"); // Some(List(List(Atom(a)),Atom(b)))
+    print sexpr.Parse("((");      // None
   }
 }
 ```
+
+A frist version of this library was implemented in pure Dafny using algebraic
+datatypes and functions. However, recursive parsing requires either late
+binding for closures or a fixpoint combinator. The latter was implemented
+correctly but simple examples caused Dafny to timeout due to the nested
+requirements of anonymous functions.
+
+Therefore, the current version is written mostly in C# with a Dafny-specific
+interface and a class/method-based API.
